theories/SScoping.v
@@ -1,6 +1,6 @@
 (* Scoping in SIRTT *)
 
-From Coq Require Import Utf8 List.
+From Coq Require Import Utf8 List Lia.
 Require Import Equations.Prop.DepElim.
 Require Import Equations.Prop.Classes.
 From Equations Require Import Equations.
@@ -479,4 +479,504 @@ Proof.
   - cbn in e. inversion e. subst. clear e.
     cbn. auto.
   - cbn in e. eapply IHh in e. auto.
+Qed.
+
+Lemma firstn_psc :
+  ∀ Γ n,
+    firstn n (psc Γ) = psc (firstn n Γ).
+Proof.
+  intros Γ n.
+  induction Γ as [| ℓ Γ ih] in n |- *.
+  - cbn. rewrite firstn_nil. reflexivity.
+  - cbn. destruct n.
+    + cbn. reflexivity.
+    + cbn. f_equal. eapply ih.
+Qed.
+
+Lemma psc_idemp :
+  ∀ Γ,
+    psc (psc Γ) = psc Γ.
+Proof.
+  induction Γ as [| ℓ Γ ih].
+  - reflexivity.
+  - cbn. rewrite pred_idemp. f_equal. auto.
+Qed.
+
+Lemma psc_app :
+  ∀ Γ Δ,
+    psc (Γ ++ Δ) = psc Γ ++ psc Δ.
+Proof.
+  intros Γ Δ.
+  induction Γ in Δ |- *.
+  - reflexivity.
+  - cbn. f_equal. eapply IHΓ.
+Qed.
+
+Lemma psc_length :
+  ∀ Γ,
+    #| psc Γ | = #| Γ |.
+Proof.
+  intros Γ. induction Γ.
+  - reflexivity.
+  - cbn. eauto.
+Qed.
+
+Inductive scoping_subst Γ : scope → list term → Type :=
+| scoping_subst_cons :
+    ∀ ℓ Δ u σ,
+      scoping Γ ℓ u →
+      scoping_subst Γ Δ σ →
+      scoping_subst Γ (ℓ :: Δ) (u :: σ)
+
+| scoping_subst_nil :
+    scoping_subst Γ [] [].
+
+Lemma scoping_subst_nth_error :
+  ∀ Γ Δ σ n ℓ u,
+    scoping_subst Γ Δ σ →
+    nth_error Δ n = Some ℓ →
+    nth_error σ n = Some u →
+    scoping Γ ℓ u.
+Proof.
+  intros Γ Δ σ n ℓ u h eΔ eσ.
+  induction h in n, ℓ, u, eΔ, eσ |- *.
+  2:{ destruct n. all: discriminate. }
+  destruct n.
+  - cbn in eΔ, eσ. inversion eΔ. inversion eσ. subst. clear eΔ eσ.
+    auto.
+  - cbn in eΔ, eσ. eapply IHh. all: eauto.
+Qed.
+
+(* Alternative where we only care about the relevant bits *)
+Inductive relevant_scoping_subst Γ : scope → list term → Type :=
+| relevant_scoping_subst_nil :
+    relevant_scoping_subst Γ [] []
+| relevant_scoping_subst_cons :
+    ∀ ℓ Δ u σ,
+      (ℓ = Level.R → scoping Γ ℓ u) →
+      relevant_scoping_subst Γ Δ σ →
+      relevant_scoping_subst Γ (ℓ :: Δ) (u :: σ).
+
+Lemma relevant_scoping_subst_nth_error :
+  ∀ Γ Δ σ n u,
+    relevant_scoping_subst Γ Δ σ →
+    nth_error Δ n = Some Level.R →
+    nth_error σ n = Some u →
+    scoping Γ Level.R u.
+Proof.
+  intros Γ Δ σ n u h eΔ eσ.
+  induction h in n, u, eΔ, eσ |- *.
+  1:{ destruct n. all: discriminate. }
+  destruct n.
+  - cbn in eΔ, eσ. inversion eΔ. inversion eσ. subst. clear eΔ eσ.
+    auto.
+  - cbn in eΔ, σ. eapply IHh. all: eauto.
+Qed.
+
+Inductive weaker_scope : scope → scope → Type :=
+| weaker_nil :
+    weaker_scope [] []
+| weaker_cons :
+    ∀ Γ Δ ℓ ℓ',
+      weaker_scope Γ Δ →
+      Level.potentially_more_relevant ℓ ℓ' →
+      weaker_scope (ℓ :: Γ) (ℓ' :: Δ).
+
+Lemma weaker_scope_nth_error :
+  ∀ Γ Δ n ℓ,
+    nth_error Δ n = Some ℓ →
+    weaker_scope Γ Δ →
+    ∑ ℓ', nth_error Γ n = Some ℓ' × Level.potentially_more_relevant ℓ' ℓ.
+Proof.
+  intros Γ Δ n ℓ e h.
+  induction h in n, ℓ, e |- *.
+  1:{ destruct n. all: discriminate. }
+  destruct n.
+  - cbn. cbn in e. inversion e. subst. clear e.
+    eexists. intuition eauto.
+  - cbn. cbn in e. eapply IHh in e. destruct e as [ℓ'' [e hℓ]].
+    eexists. intuition eauto.
+Qed.
+
+Lemma weaker_scope_psc :
+  ∀ Γ Δ,
+    weaker_scope Γ Δ →
+    weaker_scope (psc Γ) (psc Δ).
+Proof.
+  intros Γ Δ h.
+  induction h.
+  - cbn. constructor.
+  - cbn. constructor. 1: auto.
+    eapply pred_pred_le. auto.
+Qed.
+
+Lemma scoping_weak_level :
+  ∀ Γ Δ ℓ t,
+    scoping Γ ℓ t →
+    weaker_scope Δ Γ →
+    scoping Δ ℓ t.
+Proof.
+  intros Γ Δ ℓ t h hw.
+  induction h in Δ, hw |- *.
+  all: try solve [ constructor ; eauto ].
+  - eapply weaker_scope_nth_error in hw as h. 2: eauto.
+    destruct h as [ℓ' [e' hℓ]].
+    eapply scope_sub. 2: eauto.
+    constructor. auto.
+  - constructor.
+    + eapply IHh1. eapply weaker_scope_psc. auto.
+    + eapply IHh2. constructor. 1: auto.
+      right.
+  - constructor.
+    + eapply IHh1. auto.
+    + eapply IHh2. constructor. 1: auto.
+      right.
+  - constructor. 1: auto.
+    eapply IHh2. constructor. 1: auto. right.
+  - constructor. all: eauto.
+    eapply IHh1. eapply weaker_scope_psc. auto.
+  - constructor. eapply IHh. eapply weaker_scope_psc. auto.
+  - constructor. all: eauto.
+    eapply IHh1. eapply weaker_scope_psc. auto.
+  - constructor. all: eauto.
+    + eapply IHh1. eapply weaker_scope_psc. auto.
+    + eapply IHh2. eapply weaker_scope_psc. auto.
+  - constructor. all: eauto.
+    eapply IHh1. eapply weaker_scope_psc. auto.
+  - constructor. all: eauto.
+    + eapply IHh1. eapply weaker_scope_psc. auto.
+    + eapply IHh2. eapply weaker_scope_psc. auto.
+  - constructor. all: eauto.
+    eapply IHh1. eapply weaker_scope_psc. auto.
+  - eapply scope_sub. 2: eauto.
+    eapply IHh. auto.
+Qed.
+
+Lemma weaker_psc :
+  ∀ Γ,
+    weaker_scope (psc Γ) Γ.
+Proof.
+  intros Γ. induction Γ as [| ℓ Γ ih].
+  - constructor.
+  - cbn. constructor.
+    + eapply ih.
+    + eapply pred_le.
+Qed.
+
+Lemma scoping_psc :
+  ∀ Γ ℓ t,
+    scoping Γ ℓ t →
+    scoping (psc Γ) ℓ t.
+Proof.
+  intros Γ ℓ t h.
+  eapply scoping_weak_level.
+  - eauto.
+  - eapply weaker_psc.
+Qed.
+
+Lemma relevant_scoping_subst_psc :
+  ∀ Γ Δ σ,
+    relevant_scoping_subst Γ Δ σ →
+    relevant_scoping_subst (psc Γ) (psc Δ) σ.
+Proof.
+  intros Γ Δ σ h.
+  induction h.
+  - cbn. constructor.
+  - cbn. constructor. 2: eauto.
+    intro e. destruct ℓ. 2-3: discriminate.
+    cbn. eapply scoping_psc. eauto.
+Qed.
+
+Lemma scoping_ptm :
+  ∀ Γ ℓ t,
+    scoping Γ ℓ t →
+    scoping (psc Γ) (Level.pred ℓ) (ptm t).
+Proof.
+  intros Γ ℓ t h.
+  induction t in Γ, ℓ, h |- *.
+  all: try solve [ constructor ; eauto ].
+  all: try solve [ scope_inv h hs ; constructor ; intuition eauto ].
+  - scope_inv h hs. destruct hs as [ℓ' [hℓ e]].
+    eapply scope_sub.
+    + constructor. unfold psc. rewrite nth_error_map. rewrite e. cbn.
+      reflexivity.
+    + eapply pred_pred_le. auto.
+  - cbn. scope_inv h hs.
+    constructor. 1: intuition eauto.
+    eapply IHt2 with (Γ := _ :: _). intuition eauto.
+  - cbn. scope_inv h hs.
+    constructor. 1: intuition eauto.
+    rewrite max_pred. intuition eauto.
+  - cbn. scope_inv h hs.
+    constructor. 1: intuition eauto.
+    eapply IHt2 with (Γ := _ :: _). intuition eauto.
+  - cbn. scope_inv h hs. constructor. 1: intuition eauto.
+    eapply scoping_psc. intuition eauto.
+  - cbn. scope_inv h hs. destruct hs as [hs ?h].
+    eapply scope_sub.
+    + constructor. eapply scoping_psc. auto.
+    + destruct ℓ. all: cbn. 1: auto.
+      all: reflexivity.
+  - cbn. scope_inv h hs. constructor. 1: intuition eauto.
+    destruct hs as [h1 h2].
+    eapply IHt2 in h2 as ih. rewrite <- max_pred in ih.
+    auto.
+  - cbn. scope_inv h hs. constructor. all: try solve [ intuition eauto ].
+    eapply scoping_psc. intuition eauto.
+  - cbn. scope_inv h hs. constructor. all: try solve [ intuition eauto ].
+    eapply scoping_psc. intuition eauto.
+  - cbn. scope_inv h hs. constructor. 1: intuition eauto.
+    destruct hs as [h1 h2].
+    eapply IHt2 in h2 as ih. rewrite <- max_pred in ih.
+    auto.
+  - cbn. scope_inv h hs. constructor. 1: intuition eauto.
+    eapply scoping_psc. intuition eauto.
+Qed.
+
+Lemma relevant_scoping_subst_psub :
+  ∀ Γ Δ σ,
+    relevant_scoping_subst Γ Δ σ →
+    relevant_scoping_subst (psc Γ) (psc Δ) (psub σ).
+Proof.
+  intros Γ Δ σ h.
+  induction h.
+  - cbn. constructor.
+  - cbn. constructor. 2: eauto.
+    intro e. destruct ℓ. 2-3: discriminate.
+    eapply scoping_ptm. auto.
+Qed.
+
+Lemma reveal_scope_sound :
+  ∀ Γ ℓ t,
+    scoping Γ ℓ t →
+    let '(u, σ) := reveal t in
+    scoping (reveal_scope t ++ Γ) ℓ u.
+Proof.
+  fix aux 3.
+  intros Γ ℓ t h.
+  destruct t. all: try assumption.
+  - cbn. destruct l.
+    + cbn. assumption.
+    + destruct t1. all: try assumption.
+      destruct l. all: try assumption.
+      scope_inv h hs. destruct hs as [hs _].
+      scope_inv hs hs'. destruct hs' as [_ hs'].
+      eapply aux in hs'.
+      rewrite <- app_assoc. auto.
+    + destruct t1. all: try assumption.
+      destruct l. all: try assumption.
+      scope_inv h hs. destruct hs as [hs _].
+      scope_inv hs hs'. destruct hs' as [_ hs'].
+      eapply aux in hs'.
+      rewrite <- app_assoc. auto.
+  - cbn. destruct t. all: try assumption.
+    scope_inv h hs. scope_inv hs h'. destruct h' as [h' _].
+    eapply aux. auto.
+Qed.
+
+Lemma scoping_subst_app :
+  ∀ Γ Δ Ξ σ θ,
+    scoping_subst Γ Δ σ →
+    scoping_subst Γ Ξ θ →
+    scoping_subst Γ (Δ ++ Ξ) (σ ++ θ).
+Proof.
+  intros Γ Δ Ξ σ θ h1 h2.
+  induction h1 in Ξ, θ, h2 |- *.
+  - cbn. constructor. all: eauto.
+  - cbn. auto.
+Qed.
+
+Lemma scoping_subst_length :
+  ∀ Γ Δ σ,
+    scoping_subst Γ Δ σ →
+    #|σ| = #|Δ|.
+Proof.
+  intros Γ Δ σ h.
+  induction h. all: cbn ; auto.
+Qed.
+
+Lemma lift_scoping :
+  ∀ Γ Δ Ξ t ℓ,
+    scoping (Ξ ++ Γ) ℓ t →
+    scoping (Ξ ++ Δ ++ Γ) ℓ (lift #|Δ| #|Ξ| t).
+Proof.
+  intros Γ Δ Ξ t ℓ h.
+  induction t in Γ, Δ, Ξ, ℓ, h |- *.
+  all: try solve [ simpl ; constructor ].
+  all: try solve [
+    simpl ; scope_inv h hs ; constructor ; intuition eauto
+  ].
+  all: try solve [
+    simpl ; scope_inv h hs ; constructor ; intuition eauto ;
+    try lazymatch goal with
+    | h : ∀ Γ Δ Ξ ℓ, scoping _ _ ?t → _ |-
+      scoping (psc (?Ξ ++ ?Δ ++ ?Γ)) ?ℓ (lift _ _ ?t) =>
+      specialize (h (psc Γ) (psc Δ) (psc Ξ) ℓ) ;
+      rewrite !psc_app ;
+      rewrite !psc_length in h ;
+      apply h ;
+      rewrite <- !psc_app ;
+      intuition eauto
+    end ;
+    eapply IHt2 with (Ξ := _ :: _) ; intuition eauto
+  ].
+  - cbn. scope_inv h hs. destruct hs as [ℓ' [hℓ e]].
+    destruct (PeanoNat.Nat.leb_spec0 #|Ξ| n) as [h1|h1].
+    + eapply scope_sub. 2: eauto.
+      constructor.
+      rewrite nth_error_app2 in e. 2: auto.
+      rewrite nth_error_app2. 2: lia.
+      rewrite nth_error_app2. 2: lia.
+      rewrite <- e. f_equal. lia.
+    + eapply scope_sub. 2: eauto.
+      constructor. rewrite nth_error_app1 in e. 2: lia.
+      rewrite nth_error_app1. 2: lia.
+      auto.
+  - simpl. scope_inv h hs. destruct hs as [hℓ ?h].
+    eapply scope_sub. 2: eauto.
+    constructor. auto.
+Qed.
+
+Lemma weaker_scope_refl :
+  ∀ Γ,
+    weaker_scope Γ Γ.
+Proof.
+  intro Γ. induction Γ.
+  - constructor.
+  - constructor. 1: auto.
+    reflexivity.
+Qed.
+
+Lemma scoping_subst_psub :
+  ∀ Γ Δ σ,
+    scoping_subst Γ Δ σ →
+    scoping_subst (psc Γ) (psc Δ) (psub σ).
+Proof.
+  intros Γ Δ σ h.
+  induction h.
+  - cbn. constructor. 2: eauto.
+    eapply scoping_ptm. auto.
+  - cbn. constructor.
+Qed.
+
+#[local] Ltac subst_scoping_ih :=
+  lazymatch goal with
+  | h : ∀ Γ Δ Ξ ℓ σ, scoping _ _ ?t → _, hσ : scoping_subst _ ?Δ ?σ |-
+    scoping (psc (?Ξ ++ ?Γ)) ?ℓ (subst (psub ?σ) _ ?t) =>
+    specialize (h (psc Γ) (psc Δ) (psc Ξ) ℓ (psub σ)) ;
+    rewrite !psc_app ;
+    rewrite !psc_length in h ;
+    apply h ; [
+      rewrite <- !psc_app ; intuition eauto
+    | eapply scoping_subst_psub ; eauto
+    ]
+  end.
+
+Lemma subst_scoping :
+  ∀ Γ Δ Ξ ℓ σ t,
+    scoping (Ξ ++ Δ ++ Γ) ℓ t →
+    scoping_subst Γ Δ σ →
+    scoping (Ξ ++ Γ) ℓ (subst σ #|Ξ| t).
+Proof.
+  intros Γ Δ Ξ ℓ σ t ht hσ.
+  induction t in Γ, Δ, Ξ, ℓ, σ, ht, hσ |- *.
+  all: try solve [ simpl ; constructor ].
+  all: try solve [
+    simpl ; scope_inv ht hs ; constructor ; intuition eauto
+  ].
+  all: try solve [
+    simpl ; scope_inv ht hs ; constructor ; intuition eauto ;
+    eapply IHt2 with (Ξ := _ :: _) ; intuition eauto
+  ].
+  all: try solve [
+    simpl ; scope_inv ht hs ; constructor ; intuition eauto ;
+    try solve [ eapply IHt2 with (Ξ := _ :: _) ; intuition eauto ] ;
+    subst_scoping_ih
+  ].
+  - cbn. scope_inv ht hs. destruct hs as [ℓ' [hℓ e]].
+    destruct (PeanoNat.Nat.leb_spec0 #|Ξ| n) as [h1|h1].
+    + rewrite nth_error_app2 in e. 2: auto.
+      destruct (nth_error σ _) eqn:e1.
+      * eapply lift_scoping with (Ξ := []). cbn.
+        eapply nth_error_Some_length in e1 as h2.
+        eapply scoping_subst_length in hσ as eσ.
+        rewrite nth_error_app1 in e. 2: lia.
+        eapply scope_sub. 2: eauto.
+        eapply scoping_subst_nth_error. all: eauto.
+      * eapply nth_error_None in e1.
+        eapply scoping_subst_length in hσ as eσ.
+        rewrite nth_error_app2 in e. 2: lia.
+        eapply scope_sub. 2: eauto.
+        constructor. rewrite nth_error_app2. 2: lia.
+        rewrite <- e. f_equal. lia.
+    + apply PeanoNat.Nat.nle_gt in h1.
+      rewrite nth_error_app1 in e. 2: auto.
+      eapply scope_sub. 2: eauto.
+      constructor. rewrite nth_error_app1. 2: auto.
+      auto.
+  - simpl. scope_inv ht hs. destruct hs as [hℓ ?h].
+    eapply scope_sub.
+    + constructor. intuition eauto.
+    + auto.
+Qed.
+
+Lemma scoping_reveal_subst_k :
+  ∀ Γ Δ u t,
+    let '(v, σ) := reveal u in
+    scoping Γ Level.R u →
+    scoping (Δ ++ reveal_scope u ++ Γ) Level.R t →
+    scoping (Δ ++ Γ) Level.R (reveal_subst_k σ #|Δ| t).
+Proof.
+  cbn. fix aux 3. intros Γ Δ u t hu ht.
+  destruct u. all: try assumption.
+  - cbn. destruct l.
+    + assumption.
+    + destruct u1. all: try assumption.
+      destruct l. all: try assumption.
+      cbn. cbn in ht.
+      change (?t{?i := ?u})%s with (subst [u] i t).
+      scope_inv hu hs. cbn in hs. destruct hs as [hs1 hs2].
+      scope_inv hs1 hs1'.
+      eapply subst_scoping.
+      2: constructor. 3: constructor. 2: eauto.
+      cbn. eapply aux. 1: intuition eauto.
+      rewrite <- app_assoc in ht. exact ht.
+    + destruct u1. all: try assumption.
+      destruct l. all: try assumption.
+      cbn. cbn in ht.
+      change (?t{?i := ?u})%s with (subst [u] i t).
+      scope_inv hu hs. cbn in hs. destruct hs as [hs1 hs2].
+      scope_inv hs1 hs1'.
+      eapply subst_scoping.
+      2: constructor. 3: constructor. 2: eauto.
+      cbn. eapply aux. 1: intuition eauto.
+      rewrite <- app_assoc in ht. exact ht.
+  - cbn. destruct u. all: try assumption.
+    scope_inv hu hs. scope_inv hs hs'.
+    eapply aux. 1: intuition eauto.
+    cbn in ht. auto.
+Qed.
+
+Lemma scoping_reveal_subst :
+  ∀ Γ u t,
+    let '(v, σ) := reveal u in
+    scoping Γ Level.R u →
+    scoping (reveal_scope u ++ Γ) Level.R t →
+    scoping Γ Level.R (reveal_subst σ t).
+Proof.
+  cbn. intros Γ u t hu ht.
+  rewrite reveal_subst_0. eapply scoping_reveal_subst_k with (Δ := []).
+  all: auto.
+Qed.
+
+Lemma skipn_psc :
+  ∀ Γ n,
+    skipn n (psc Γ) = psc (skipn n Γ).
+Proof.
+  intros Γ n.
+  induction Γ as [| ℓ Γ ih] in n |- *.
+  - cbn. rewrite skipn_nil. reflexivity.
+  - cbn. destruct n.
+    + cbn. reflexivity.
+    + cbn. eapply ih.
 Qed.
